EnvTy.v
@@ -1,0 +1,127 @@
+Require Import Var Val Env Map.
+
+Import BMap.
+
+Set Implicit Arguments.
+
+Open Scope map_scope.
+(** * Types for Environments *)
+
+Definition envOfType (E:env val) (ET:onv ty) : Prop := 
+  forall x t, ET[x]= Some t -> valOfType (E[x]) t.
+
+(** Stability under typed update *)
+Lemma envOfType_update E (ET:onv ty) (ETd:envOfType E ET) v t (vtd:valOfType v t) x
+  : envOfType (E[x<-v]) (ET[x<-Some t]).
+Proof.
+  intros y t'. destruct_prop (x==y); eqsubst; subst. 
+  simplify lookup; intros; try congruence.
+  simplify lookup; eauto.
+Qed.
+
+(** Anything is well typed under the empty environment *)
+Lemma envOfType_empty E
+  : envOfType E (ompty ty).
+Proof.
+  intros x t neq. cbv in neq. rewrite empty_spec in neq. congruence.
+Qed.
+
+(** ** A relation characterizing sub-environment *) 
+
+Definition subEnv Y (E E':onv Y)
+  := forall x y, E[x] = Some y -> E'[x] = Some y.
+
+Lemma subEnv_refl Y (E:onv Y)
+  : subEnv E E.
+Proof.
+  firstorder.
+Qed.
+
+Lemma subEnv_empty Y (E:onv Y)
+  : subEnv (ompty Y) E.
+Proof.
+  hnf; intros. cbv in H. rewrite empty_spec in H. congruence.
+Qed.
+
+Lemma envOfType_weakening E ET ET'
+  : subEnv ET ET' -> envOfType E ET' -> envOfType E ET.
+intros A B x t eq. eauto.
+Qed.
+
+Lemma subEnv_update Y (ET ET':onv Y) x y
+  : subEnv ET ET' -> subEnv (ET[x<-y]) (ET'[x<-y]).
+Proof.
+  intros; hnf; intros. destruct_prop (x=x0); subst; simplify lookup; eauto.
+Qed.
+
+Lemma subEnv_trans Y (ET ET' ET'':onv Y)
+  : subEnv ET ET' -> subEnv ET' ET'' -> subEnv ET ET''.
+Proof.
+  intros; hnf; intros. firstorder.
+Qed.
+
+(** ** Environment Equivalence at an environemnt type *)
+
+Definition typed_eq {X Y:Type} `(Defaulted X) (ET:onv Y) (E E': env X) :=
+  forall x t, ET[x] = Some t -> E[x] = (E'[x]).
+
+
+Lemma typed_eq_refl (X Y:Type) `(Defaulted X) (ET:onv Y) : forall (E:env X), typed_eq ET E E.
+  firstorder.
+Qed.
+
+Hint Resolve typed_eq_refl.
+
+Global Instance typed_eq_Refl {X Y Z:Type} {ET:onv Y} `{Defaulted X}
+  : Reflexive (typed_eq ET) := @typed_eq_refl X Y _ ET.
+
+Lemma typed_eq_sym X Y Z ET : forall E E', @typed_eq X Y Z ET E E' -> typed_eq ET E' E.
+  hnf. unfold typed_eq. intros. symmetry; eauto.
+Qed.
+
+Hint Resolve typed_eq_sym.
+
+Global Instance typed_eq_Sym {X Y ET} `{Defaulted X} : Symmetric (typed_eq ET) := 
+  @typed_eq_sym X Y _ ET.
+
+Lemma typed_eq_trans X Y Z ET : forall E E' E'',
+  @typed_eq X Y Z ET E E' -> typed_eq ET E' E'' -> typed_eq ET E E''.
+  hnf. unfold typed_eq. intros. erewrite H; eauto.
+Qed.
+
+Global Instance typed_eq_Trans {X Y ET} `{Defaulted X} : Transitive (typed_eq ET) := 
+  @typed_eq_trans X Y _ ET.
+
+
+Lemma typed_eq_update Y (ET:onv Y) (E E':env val) (y:Y) x z 
+  : typed_eq ET E E' -> typed_eq (ET [x <- Some y]) (E [x <- z]) (E' [x <- z]).
+Proof.
+  intros A a t eq. destruct_prop (a == x); eqsubst; subst.
+  simplify lookup; eauto.
+  simplify lookup; eauto.
+Qed.
+
+Lemma typed_eq_empty (Y:Type) (E E':env val)
+  : typed_eq (ompty Y) E E'.
+Proof.
+  intros x t neq. cbv in neq. rewrite empty_spec in neq. congruence.
+Qed.
+
+Lemma typed_eq_envOfType ET E E'
+  : typed_eq ET E E' -> envOfType E ET -> envOfType E' ET.
+Proof.
+  intros A B x t eq. erewrite <- A; eauto.
+Qed.
+
+Lemma typed_eq_weakening Y (ET ET': onv Y) (E E':env val)
+  : typed_eq ET E E' -> subEnv ET' ET -> typed_eq ET' E E'.
+Proof.
+  intros A B x t eq. eauto.
+Qed.
+
+
+(* 
+*** Local Variables: ***
+*** coq-load-path: ("infra" "constr" "il" "isa" ".") ***
+*** End: ***
+*)
