constr/CSet.v
@@ -57,6 +57,15 @@ Module Type CSet.
   Definition incl X (s t:cset X) :=
     forall x, member x s -> member x t. 
 
+  Parameter size : forall X : Type, cset X -> nat.
+
+  Parameter size_spec : forall X (s : cset X), size s = length (elements s).
+(*
+  Parameter set_ind
+    : forall X (P:cset X -> Prop), P empty 
+      -> (forall (x:X) (s:cset X), P s -> ~member x s -> P (join (single x) s))
+      -> forall s:cset X, P s.
+*)
 End CSet.
 
 Module Type CSetNotation (Import M : CSet).
@@ -180,6 +189,11 @@ Module BSet <: CSet.
   Parameter elements_spec
     : forall X (s:cset X) x, member x s <-> List.In x (elements s).
 
+  Parameter size : forall X : Type, cset X -> nat.
+
+  Parameter size_spec : forall X (s : cset X), size s = length (elements s).
+
+
   Include CSetNotation.
   Include CSetEquality.
  
@@ -229,7 +243,7 @@ Module BSet <: CSet.
     cset_tac; firstorder.
   Qed.
 
-  Lemma in_add_case X `(EqDec X eq) s (x y:X)
+  Lemma in_add_case X `{EqDec X eq} s (x y:X)
     : y ∈ {{x}} ∪ s -> x=y \/ (x<>y /\ y ∈ s).
   Proof.
     destruct_prop (x=y); cset_tac; firstorder.
@@ -279,6 +293,37 @@ Module BSet <: CSet.
     repeat (cset_tac; subst; firstorder).
   Qed.
 
+  Lemma not_in_empty X (x:X)
+    : x ∉ ∅.
+  Proof.
+    cset_tac; firstorder.
+  Qed.
+
+
+  Lemma minus_inane_set X (s t:cset X)
+    : s ∩ t = ∅ -> (s \ t) = s.
+  Proof.
+    cset_tac; firstorder.
+    eapply (not_in_empty x). rewrite <- H.
+    cset_tac; firstorder.
+  Qed.
+
+  Lemma minus_union_set X (s t:cset X)
+    : s ∩ t = ∅ -> ((s ∪ t) \ t) = s.
+  Proof.
+    cset_tac; firstorder.
+    eapply (not_in_empty x). rewrite <- H.
+    cset_tac; firstorder.
+  Qed.
+
+
+  Lemma in_minus_neq X s (x y:X)
+    : x <> y -> x ∈ s
+    -> x ∈ (s\{{y}}).
+  Proof.
+    repeat (cset_tac; subst; firstorder).
+  Qed.
+
   Lemma add_inane X s (x:X) 
     : x ∈ s
     -> s = ({{x}} ∪ s).
@@ -305,7 +350,6 @@ Module BSet <: CSet.
   Qed.
 
 
-
   Lemma incl_trans X (s t u:cset X)
     : incl s t -> incl t u -> incl s u.
   Proof.
@@ -313,7 +357,7 @@ Module BSet <: CSet.
   Qed.
 
   Lemma minus_incl X (s t:cset X)
-    : incl (s\t) s.
+    : (s\t) ⊆ s.
   Proof.
     hnf; cset_tac; firstorder.
   Qed.
@@ -338,8 +382,8 @@ Module BSet <: CSet.
   Qed.
 
 
-  Lemma incl_minus_single X s (x:X)
-    :  incl (s \ {{x}}) s.
+  Lemma incl_minus X (s t : cset X)
+    :  incl (s \ t) s.
   Proof.
     hnf; cset_tac; firstorder.
   Qed.
@@ -371,8 +415,15 @@ Module BSet <: CSet.
     hnf; cset_tac; firstorder.
   Qed.
 
-  Lemma union_idem X (s t:cset X)
-    : s ∪ s ∪ t = s ∪ t.
+  Lemma incl_minus_lr X (s s' t t':cset X)
+    : s ⊆ s' -> t ⊆ t' -> s \ t' ⊆ s' \ t.
+  Proof.
+    intros; hnf in *; hnf; cset_tac; firstorder.
+  Qed.
+
+
+  Lemma union_idem X (s:cset X)
+    : s ∪ s = s.
   Proof.
     hnf; cset_tac; firstorder.
   Qed.
@@ -405,6 +456,12 @@ Module BSet <: CSet.
 
   Lemma union_cases X s t (x:X)
     : x ∈ (s ∪ t) -> x ∈ s \/ x ∈ t.
+  Proof.
+    cset_tac; firstorder.
+  Qed.
+
+  Lemma not_in_union_comp A (s t : cset A) x :
+    ~x ∈ s /\ ~x ∈ t -> ~x ∈ (s ∪ t).
   Proof.
     cset_tac; firstorder.
   Qed.
@@ -460,7 +517,567 @@ Module BSet <: CSet.
     intros; hnf in *; hnf; cset_tac; firstorder.
   Qed.
 
+  Lemma incl_union_lr X (s s' t t':cset X)
+    : s ⊆ s' -> t ⊆ t' -> s ∪ t ⊆ s' ∪ t'.
+  Proof.
+    intros; hnf in *; hnf; cset_tac; firstorder.
+  Qed.
+
+
+  Lemma incl_not_in X (ED:EqDec X eq) (x:X) s t
+    : x ∉ s -> s\{{x}} ⊆ t -> s ⊆ t.
+  Proof.
+    intros; hnf; intros. eapply H0.
+    destruct_prop (x0=x); subst.
+    exfalso. eauto.
+    eapply in_in_minus; eauto. cset_tac; firstorder.
+  Qed.
+
+  Lemma incl_left X (s t:cset X)
+    : s ⊆ (s ∪ t).
+  Proof.
+    hnf; intros. cset_tac; firstorder.
+  Qed.
+
+  Lemma in_meet X (s t:cset X) (x:X)
+    : x ∈ s -> x ∈ t -> x ∈ s ∩ t.
+  Proof.
+    cset_tac; firstorder.
+  Qed.
+
+  Lemma meet_in X (s t:cset X) (x:X)
+    : x ∈ s ∩ t -> x ∈ s /\ x ∈ t.
+  Proof.
+    cset_tac; firstorder.
+  Qed.
+
+  Lemma meet_incl X (s t u:cset X) 
+    : s ⊆ u -> s ∩ t ⊆ u.
+  Proof.
+    intros; hnf in *; cset_tac; firstorder.
+  Qed.
+
+  Lemma meet_comm X (s t:cset X)
+    : s ∩ t = t ∩ s.
+  Proof.
+    cset_tac; firstorder.
+  Qed.
+
+  Lemma incl_meet X (s t:cset X)
+    : s ⊆ t -> s = s ∩ t.
+  Proof.
+    repeat (cset_tac; subst; firstorder).
+  Qed.
+
+  Lemma incl_refl X (s:cset X)
+    : s ⊆ s.
+  Proof.
+    firstorder.
+  Qed.
+
+  Lemma minus_meet X (s t u:cset X)
+    : (s \ t) ∩ u = s ∩ u \ t.
+  Proof.
+    cset_tac; firstorder.
+  Qed.
+
+  Lemma set_incl X (s t: cset X)
+    : s ⊆ t -> t ⊆ s -> t = s.
+  Proof.
+    intros; hnf in *; cset_tac; firstorder.
+  Qed.
+
+
+  Lemma elements_nil_eset {X : Type} (s : cset X) :
+    s = ∅ <-> elements s = nil.
+  Proof.
+    split; intros.
+    rewrite H; clear H.
+    remember (@elements X ∅) as l.
+    destruct l.
+    reflexivity.
+    assert (In x (x :: l)) by (apply in_eq).
+    rewrite Heql in H.
+    rewrite <- elements_spec in H.
+    cset_tac. inversion H.
+
+    specialize (elements_spec s); intros.
+    rewrite H in H0. simpl in H0.
+    cset_tac. specialize (H0 x). tauto. inv H1.
+  Qed.
+
+  Lemma fromList_elements X :
+    forall s, fromList (@elements X s) = s.
+  Proof.
+    cset_tac. rewrite in_fromList in H. rewrite elements_spec. assumption.
+    rewrite in_fromList. rewrite elements_spec in H. assumption.
+  Qed.
+
+  Lemma elements_fromList_in X (l : list X) x :
+    In x l <-> In x (elements (fromList l)).
+  Proof.
+    split; intros.
+    rewrite <- elements_spec.
+    rewrite in_fromList; assumption.
+    rewrite <- elements_spec in H.
+    rewrite in_fromList in H; assumption.
+  Qed.
+
+  Lemma fromList_eq X :
+    forall l l', l = l' -> @fromList X l = @fromList X l'.
+  Proof.
+    intros.
+    destruct l, l'; try (inversion H); try reflexivity.
+  Qed.
+
+  Lemma forallb_add {X : Type} {ED:EqDec X eq} (s : cset X) (f : X -> bool) (x : X) : 
+    BSet.forallb ({{x}} ∪ s) f = (f x) && (BSet.forallb s f).
+  Proof.
+    apply eq_bool_prop_intro.
+    intros; split; intros.
+    rewrite forallb_spec in H.
+    bool_to_prop. split.
+    eapply H. cset_tac; firstorder.
+    rewrite forallb_spec.
+    intros.
+    eapply H. cset_tac; firstorder.
+
+    bool_to_prop in H.
+    invc H.
+    rewrite forallb_spec.
+    intros.
+    destruct_prop (x = x0). subst x0; assumption.
+    cset_tac. firstorder.
+    rewrite forallb_spec in H1.
+    eauto.
+  Qed.
+
+  Lemma forallb_false {X : Type} {ED:EqDec X eq} (s : cset X) (f : X -> bool) :
+    BSet.forallb s f = false <-> exists x, x ∈ s /\ f x = false.
+  Proof.
+    rewrite <- negb_true_iff.
+    remember (elements s) as l.
+    specialize (elements_unique s); intro Huniq.
+    rewrite <- Heql in Huniq.
+    simpl in Huniq.
+    apply fromList_eq in Heql.
+    generalize dependent s.
+    induction l; intros; split; intros.
+
+    apply Is_true_eq_left in H; bool_to_prop in H; 
+       symmetry in Heql; simpl in Heql; rewrite fromList_elements in Heql.
+    subst s. rewrite forallb_spec in H. exfalso. apply H. intros. cset_tac. inv H0.
+    apply Is_true_eq_true; bool_to_prop;
+    symmetry in Heql; simpl in Heql; rewrite fromList_elements in Heql.
+    intro. subst s. cset_tac. inv H2.
+
+    simpl in Heql.
+    rewrite fromList_elements in Heql.
+    specialize (IHl (snd Huniq) (fromList l)).
+    rewrite fromList_elements in IHl.
+    specialize (IHl (eq_refl (fromList l))).
+
+    rewrite <- Heql in H.
+    rewrite forallb_add in H.
+    rewrite negb_andb in H.
+    apply orb_true_iff in H.
+    rewrite negb_true_iff in H.
+    inversion H.
+    exists a. split.
+    rewrite <- Heql.
+    apply in_single_union.
+    assumption.
+
+    apply IHl in H0.
+    inversion H0.
+    exists x.
+    invc H1.
+    split; [ eapply union_right | idtac ]; assumption.
+    
+    inversion H.
+    invc H0.
+    apply Is_true_eq_true.
+    bool_to_prop; intro.
+    rewrite forallb_spec in H0.
+    specialize (H0 x H1).
+    apply Is_true_eq_true in H0.
+    rewrite H2 in H0.
+    inversion H0.
+  Qed.
+
+  Lemma forallb_eq_funs {X : Type} (s : cset X) (f g : X -> bool) :
+    (forall x, x ∈ s -> f x = g x) -> BSet.forallb s f = BSet.forallb s g.
+  Proof.  
+    intros.
+    apply eq_bool_prop_intro.
+    repeat rewrite forallb_spec.
+    split; intros;
+    specialize (H x H1); specialize (H0 x H1); [ rewrite <- H | rewrite H ]; assumption.
+  Qed.
+
+  Lemma not_empty_contains_element {X : Type} (s : cset X) :
+    s <> ∅ <-> exists x, x ∈ s.
+  Proof.
+    split; intros.
+    remember (elements s) as l.
+    generalize dependent s.
+    destruct l; intros.
+    exfalso. apply H. apply elements_nil_eset. symmetry. assumption.
+    specialize (@fromList_elements X s); intros.
+    rewrite <- Heql in H0. simpl in H0.
+    rewrite <- H0.
+    exists x.
+    apply in_single_union.
+
+    cset_tac; firstorder.
+  Qed.
+
+  (*
+  Lemma not_empty_split {X : Type} (s : cset X) :
+    s <> ∅ <-> exists x, exists s', ~ x ∈ s' /\ s = {{x}} ∪ s'.
+  Proof.
+    split; intros.
+    apply not_empty_contains_element in H.
+    invc H.
+    exists x.
+    exists (s \ {{x}}).
+    split. cset_tac; firstorder.
+    eapply incl_set_decomp.
+    unfold incl.
+    intros.
+    cset_tac. invc H; [ subst; assumption | firstorder ].
+  
+    invc H. invc H0. invc H. intro. apply H0.
+    rewrite elements_nil_eset in H.
+    specialize (elements_spec ({{x}} ∪ x0)); intros.
+    specialize (H1 x).
+    rewrite H in H1.
+    exfalso. eapply in_nil. apply H1. cset_tac; firstorder.
+  Qed.
+  *)
+
+  Lemma union_meet_distr_r {A} (s t u : cset A) :
+    (s ∪ t) ∩ u = (s ∩ u) ∪ (t ∩ u).
+  Proof.
+    cset_tac; firstorder.
+  Qed.
+
+  Lemma union_is_empty {A} (s t : cset A) :
+    s ∪ t = ∅ -> (s = ∅ /\ t = ∅).
+  Proof.
+    cset_tac; firstorder.
+    apply (union_left s t) in H0. rewrite H in H0. rewrite empty_spec in H0. assumption.
+    apply (union_left t s) in H0. rewrite union_comm in H0. rewrite H in H0. rewrite empty_spec in H0. assumption.
+  Qed.
+
+  Lemma smaller_meet_empty {A} (s t u : cset A) :
+    (s ∪ t) ∩ u = ∅ -> t ∩ u = ∅.
+  Proof.
+    intros. cset_tac. 
+    rewrite union_meet_distr_r in H.
+    specialize (in_meet t u x H1 H2); intros.
+    apply union_is_empty in H. invc H. rewrite H4 in H0. rewrite empty_spec in H0. assumption.
+    inv H0. inv H0.
+  Qed.
+
+  Lemma empty_intersection_in_one_not_other {A} (s t : cset A) x :
+    s ∩ t = ∅ -> x ∈ s -> ~ x ∈ t.
+  Proof.
+    cset_tac. apply (not_in_empty x). rewrite <- H. apply in_meet; assumption.
+  Qed.
+
+  Lemma not_empty_split {X : Type} (s : cset X) :
+    s <> ∅ <-> exists x, exists s', ~ x ∈ s' /\ s = {{x}} ∪ s'.
+  Proof.
+    split; intros.
+    apply not_empty_contains_element in H.
+    inversion H; clear H.
+    exists x.
+    exists (s \ {{x}}).
+    split. cset_tac; firstorder.
+    eapply incl_set_decomp.
+    unfold incl.
+    intros.
+    hnf; repeat (cset_tac; firstorder).
+  
+    cset_tac; firstorder.
+    rewrite elements_nil_eset in H.
+    specialize (elements_spec ({{x}} ∪ x0)); intros.
+    specialize (H1 x).
+    unfold add in H1. rewrite H in H1.
+    exfalso. eapply in_nil. apply H1. cset_tac; firstorder.
+  Qed.
+
+  Lemma meet_assoc X (s t u : cset X)
+    : s ∩ t ∩ u = s ∩ (t ∩ u).
+  Proof.
+    cset_tac; firstorder.
+  Qed.
+
+  Lemma incl_meet_lr X (s s' t t':cset X)
+    : s ⊆ s' -> t ⊆ t' -> s ∩ t ⊆ s' ∩ t'.
+  Proof.
+    intros; hnf in *; hnf; cset_tac; firstorder.
+  Qed.
+
+
+
+
+
+
+
+
+
+
+
+
+
+
+  Lemma unique_remove {A : Type} (p q : list A) (x : A) :
+    unique (p ++ x :: q) -> unique (p ++ q).
+  Proof.
+    induction p; simpl in *; intros. apply (snd X).
+    specialize (IHp (snd X)).
+    constructor.
+    intro.
+    apply (fst X).
+    apply in_app_or in H.
+    apply in_or_app.
+    inversion H; auto. right. simpl. right. assumption.
+    assumption.
+  Qed.
+
+  Lemma unique_replace {A : Type} (p q : list A) (x y : A) :
+    unique (p ++ x :: q) ->
+    ~ In y p ->
+    ~ In y q ->
+    unique (p ++ y :: q).
+  Proof.
+    intros.
+    generalize dependent y.
+    generalize dependent q.
+    induction p; intros; simpl in *; constructor.
+    apply H0. apply (snd X).
+    intro.
+    apply in_app_or in H1.
+    firstorder.
+
+    apply IHp.
+    apply (snd X).
+    firstorder.
+    assumption.
+  Qed.   
+
+  Lemma unique_split {A : Type} (p q : list A) (x : A) :
+    unique (p ++ x :: q) -> (~ In x p /\ ~ In x q).
+  Proof.
+    intros.
+    induction p.
+    simpl in *.
+    split; auto. apply (fst X).
+    simpl in X.
+    specialize (IHp (snd X)).
+    inversion IHp.
+    split; intro.
+    apply H. simpl in H1. inversion H1. subst x.
+    exfalso. apply (fst X).
+    apply in_or_app. right. simpl. auto.
+    assumption.
+    auto.
+  Qed.
+
+  Lemma length_unique_eq {A : Type} `{EqDec A eq} (l l' : list A) :
+    unique l ->
+    unique l' ->
+    (forall x, In x l <-> In x l') ->
+    length l = length l'.
+  Proof.
+    intros.
+    generalize dependent l'.
+    induction l; intros.
+    destruct l'.
+    reflexivity.
+    exfalso.
+    simpl in H0.
+    rewrite H0.
+    left. apply (eq_refl a).
+
+    destruct l'; simpl in *.
+    exfalso. rewrite <- H0. left; apply (eq_refl a).
+
+    destruct_prop (a = a0).
+    subst a0. f_equal.
+    apply IHl. apply (snd X). apply (snd X0).
+    intros; rewrite <- or_cancel_l.
+    apply H0.
+    intros. intro. apply (fst X). subst a; assumption.
+    intros. intro. apply (fst X0). subst a; assumption.
+
+    assert (In a l') by firstorder.
+    apply in_split in H1.
+    inversion H1 as [p [q Hpq]]; clear H1.
+
+    assert (length (p ++ a0 :: q) = length l').
+    rewrite Hpq.
+    repeat rewrite app_length.
+    f_equal.
+    rewrite <- H1.
+    f_equal.
+    apply IHl.
+    apply (snd X).
+    eapply unique_replace.
+    assert (unique (p ++ a :: q)) by (rewrite <- Hpq; apply (snd X0)).
+    apply X1.
+    intro. apply (fst X0). rewrite Hpq. apply in_or_app. auto.
+    intro. apply (fst X0). rewrite Hpq. apply in_or_app. right. apply in_cons. assumption.
+    
+    intros; split; intros; specialize (H0 x).
+    specialize (fst X); intros. unfold fresh in X1.
+    destruct_prop (a0 = x); apply in_or_app.
+    subst x. right. apply in_eq.
+    assert (In x l') by firstorder.
+    rewrite Hpq in H3.
+    apply in_app_or in H3.
+    inversion H3. left. assumption. right.
+    simpl in H4.
+    inversion H4.
+    subst a. absurd (In x l); assumption.
+    apply in_cons. assumption.
+
+    assert (x <> a).
+    intro. apply (fst X).
+    subst x.
+    apply in_app_or in H2.
+    assert (~ In a p /\ ~ In a q).
+    apply unique_split. rewrite <- Hpq. apply (snd X0).
+    inversion H3. clear H3.
+    inversion H2. contradiction.
+    simpl in H3. exfalso; firstorder.
+    
+    destruct_prop (a0 = x). firstorder.
+    assert (In x (p ++ a :: q)).
+    apply in_app_or in H2.
+    inversion H2. apply in_or_app. left. assumption.
+    simpl in H4.
+    inversion H4. absurd (a0 = x); assumption.
+    apply in_or_app. right. simpl. right. assumption.
+    rewrite <- Hpq in H4.
+    firstorder.
+  Qed.
+
+  Lemma fromList_size {A : Type} `{EqDec A eq} (p : list A) :
+    unique p -> size (fromList p) = length p.
+  Proof.
+    induction p; intros. simpl in *.
+    rewrite size_spec.
+    assert (@elements A ∅ = nil). rewrite <- (elements_nil_eset ∅). reflexivity. 
+    rewrite H0. reflexivity.
+
+    symmetry.
+    rewrite size_spec.
+    eapply length_unique_eq.
+    assumption.
+    eapply elements_unique.
+    apply elements_fromList_in.
+  Qed.
+  
+  Lemma fromList_drop {A : Type} (p q : list A) (x : A) : 
+    unique (p ++ x :: q) ->
+    fromList (p ++ q) = fromList (p ++ x :: q) \ {{x}}.
+  Proof.
+    intros.
+    induction p; simpl in *.
+
+    erewrite <- union_minus. reflexivity.
+    rewrite in_fromList.
+    apply (fst X).
+
+    specialize (IHp (snd X)).
+    rewrite IHp.
+    repeat (cset_tac; firstorder).
+  Qed.
+
+  Lemma fromList_drop' {A : Type} (q : list A) (x : A) :
+    unique (x :: q) -> fromList q = fromList (x :: q) \ {{x}}.
+  Proof.
+    intros.
+    assert (fromList (nil ++ q) = fromList (nil ++ x :: q) \ {{x}}).
+    apply fromList_drop.
+    assumption.
+    assumption.
+  Qed.
+
+  Lemma size_add_disjoint {A : Type} `{EqDec A eq} (s : cset A) (x : A) :
+    ~ (x ∈ s) -> size ({{x}} ∪ s) = S (size s).
+  Proof.
+    intros.
+    assert (In x (elements ({{x}} ∪ s))).
+    apply elements_spec. repeat (cset_tac; firstorder).
+    apply in_split in H1.
+    inversion H1 as [p [q Hpq]]; clear H1.
+    specialize (elements_unique ({{x}} ∪ s)); intros H1.
+    rewrite Hpq in H1.
+    apply fromList_eq in Hpq. rewrite fromList_elements in Hpq.
+    assert (s = fromList (p ++ q)).
+    apply fromList_drop in H1.
+    rewrite H1. rewrite <- Hpq. rewrite <- union_minus. reflexivity. assumption.
+    rewrite Hpq. rewrite H2.
+    repeat rewrite fromList_size.
+    repeat rewrite app_length. simpl. omega.
+    eapply unique_remove. apply H1. assumption.
+  Qed.
+
+
+  Lemma cset_ind {A : Type} `{EqDec A eq} (P : cset A -> Prop) :
+    P ∅ ->
+    (forall s x, P s -> ~ x ∈ s -> P ({{x}} ∪ s)) ->
+    forall s, P s.
+  Proof.
+    intros.
+
+    assert (exists l, (forall x, In x l <-> x ∈ s) /\ exists t : unique l, True).
+    exists (elements s). split. intros; rewrite elements_spec. reflexivity.
+    exists (elements_unique s). constructor.
+
+    inversion H2 as [l Hl]; clear H2.
+    generalize dependent s.
+    induction l; intros.
+    simpl in Hl.
+    assert (s = ∅) by (cset_tac; firstorder).
+    subst s; assumption.
+
+    inversion Hl; clear Hl.
+    inversion H3 as [Hu Hgigo]; clear Hgigo H3.
+    assert (s = fromList (a :: l)).
+    apply set_extensionality; intros; apply eq_bool_prop_intro.
+    rewrite <- H2. rewrite <- in_fromList. reflexivity.
+
+    specialize (fromList_drop' Hu); intros.
+    rewrite <- H3 in H4.
+    assert (a ∈ s) by (simpl in H2; cset_tac; firstorder).
+    assert (s = {{a}} ∪ (fromList l)).
+    rewrite H4.
+    cset_tac.
+    destruct_prop (x = a). firstorder. right. firstorder.
+    invc H3. invc H6. assumption. contradiction. tauto.
+    
+    rewrite H6.
+    apply H1; try assumption.
+    apply IHl.
+    split.
+    symmetry. apply in_fromList.
+    exists (snd Hu).
+    constructor.
+
+    rewrite H4.
+    cset_tac; firstorder.
+  Qed.
+
+
+
 End BSet.
+
+                  
 
 
 (* 
