isa/Exp.v
@@ -1,4 +1,4 @@
-Require Import Util Val Env.
+Require Import Util Val Env EnvTy liveness_fwd.
 
 Set Implicit Arguments.
 
@@ -12,6 +12,21 @@ Set Implicit Arguments.
   Variable exp : Type.
   Hypothesis exp_eval : env val -> exp -> option val .
   Hypothesis expOfType : onv ty -> exp -> ty -> Prop.
+  Hypothesis expOfType_subEnv 
+    : forall ET ET' e t, subEnv ET' ET -> expOfType ET' e t -> expOfType ET e t.
+  Hypothesis exp_type_soundness : forall ET E e t, expOfType ET e t -> envOfType E ET ->
+    { v : val & ((exp_eval E e = Some v) * valOfType v t)%type }.
+  Hypothesis exp_eval_typed_eq 
+    : forall ET E E' e t, typed_eq ET E E' -> expOfType ET e t 
+      -> exp_eval E e = exp_eval E' e.
+
+  Hypothesis live_exp_sound : exp -> live -> Type.
+  Hypothesis live_exp_sound_incl 
+    : forall e lv lv', lv' ⊆ lv -> live_exp_sound e lv' -> live_exp_sound e lv.
+
+  Hypothesis exp_eval_live 
+    : forall e lv E E', live_exp_sound e lv -> agree_on lv E E' -> 
+      exp_eval E e = exp_eval E' e.
 
   Hypothesis var_to_exp : forall x:var, exp.
   Hypothesis var_to_exp_correct : forall M x,
