liveness_fwd.v
@@ -1,0 +1,11 @@
+Require Import List CSet.
+Require Export Env.
+
+Export BSet.
+
+Open Scope cset_scope.
+
+Set Implicit Arguments.
+
+Definition live := BSet.cset var.
+
